for RW

concurrency/framework/PCMWrap.s.dfy
@@ -1,6 +1,8 @@
 include "PCM.s.dfy"
 
 abstract module PCMWrap refines PCM {
+  import opened GhostLoc
+
   /*abstract*/ type G(!new)
 
   datatype M = M(ghost m: multiset<G>)
@@ -10,22 +12,16 @@ abstract module PCMWrap refines PCM {
 
   function unit() : M { nil() }
 
-  predicate {:extern} dot_defined(x: M, y: M)
-  function {:extern} dot(x: M, y: M) : M
-  lemma {:extern} dot_unit(x: M)
-  lemma {:extern} commutative(x: M, y: M)
-  lemma {:extern} associative(x: M, y: M, z: M)
-  lemma {:extern} transition_is_monotonic(a: M, b: M, c: M)
+  function dot(x: M, y: M) : M { M(x.m + y.m) }
 
   predicate transition(a: M, b: M) { a == b }
 
-  function singleton_loc(): Loc
+  lemma dot_unit(x: M) { }
+  lemma commutative(x: M, y: M) { }
+  lemma associative(x: M, y: M, z: M) { }
+  lemma transition_is_monotonic(a: M, b: M, c: M) { }
 
-  type GToken = t : Token | t.loc == singleton_loc()
-    witness *
-
-  function method {:extern} wrap(glinear g: G) : (glinear t: GToken)
-  ensures t.val == one(g)
+  function {:extern} singleton_loc(): Loc
 
   predicate is_one(m: M) {
     exists a :: m == one(a)
@@ -36,13 +32,23 @@ abstract module PCMWrap refines PCM {
   {
     var a :| m == one(a); a
   }
+}
+
+module PCMWrapTokens(pcm: PCMWrap) {
+  import T = Tokens(pcm)
+  type G = pcm.G
+
+  type GToken = t : T.Token | t.loc == pcm.singleton_loc()
+    witness *
+
+  function method {:extern} wrap(glinear g: G) : (glinear t: GToken)
+  ensures t.val == pcm.one(g)
 
   function method {:extern} unwrap(glinear t: GToken) : (glinear g: G)
-  requires is_one(t.val)
-  ensures g == get_one(t.val)
+  requires pcm.is_one(t.val)
+  ensures g == pcm.get_one(t.val)
 
   function method {:extern} unwrap_borrow(gshared t: GToken) : (gshared g: G)
-  requires is_one(t.val)
-  ensures g == get_one(t.val)
-
+  requires pcm.is_one(t.val)
+  ensures g == pcm.get_one(t.val)
 }
