concurrency/framework/RwSSM.i.dfy
@@ -1,9 +1,14 @@
 include "PCM.s.dfy"
+include "PCMExt.s.dfy"
+include "PCMWrap.s.dfy"
+include "../../lib/Base/Option.s.dfy"
 
-abstract module RwPCM {
-  type StoredType
+abstract module RW {
+  import opened Options
 
-  type M
+  type StoredType(!new)
+
+  type M(!new)
 
   function dot(x: M, y: M) : M
   function unit() : M
@@ -13,7 +18,27 @@ abstract module RwPCM {
   function I(x: M) : Option<StoredType> requires Inv(x)
 
   predicate transition(a: M, b: M) {
-    forall p :: Inv(dot(a, p)) ==> Inv(dot(b, p)) && I(dot(a, p)) == I(dot(b, p))
+    forall p: M :: Inv(dot(a, p)) ==> Inv(dot(b, p)) && I(dot(a, p)) == I(dot(b, p))
+  }
+
+  predicate deposit(a: M, b: M, x: StoredType)
+  {
+    forall p: M :: Inv(dot(a, p)) ==> Inv(dot(b, p))
+        && I(dot(a, p)) == None
+        && I(dot(b, p)) == Some(x)
+  }
+
+  predicate withdraw(a: M, b: M, x: StoredType)
+  {
+    forall p: M :: Inv(dot(a, p)) ==> Inv(dot(b, p))
+        && I(dot(a, p)) == Some(x)
+        && I(dot(b, p)) == None
+  }
+
+  predicate borrow(a: M, x: StoredType)
+  {
+    forall p: M :: Inv(dot(a, p)) ==>
+        && I(dot(a, p)) == Some(x)
   }
 
   lemma dot_unit(x: M)
@@ -25,22 +50,127 @@ abstract module RwPCM {
   lemma associative(x: M, y: M, z: M)
   ensures dot(x, dot(y, z)) == dot(dot(x, y), z)
 
-  lemma exists_inv_state()
-  returns (s: M)
-  ensures Inv(s)
+  lemma InitImpliesInv(x: M)
+  requires Init(x)
+  ensures Inv(x)
+  ensures I(x) == None
+
+  // TODO(travis) I think this is probably unnecessary
+  // For now, just add "or m == unit()" to your Invariant.
+  lemma inv_unit()
+  ensures Inv(unit())
+  ensures I(unit()) == None
+}
+
+module RW_PCMWrap(rw: RW) refines PCMWrap {
+  type G = rw.StoredType
+}
+
+module RW_PCMExt(rw: RW) refines PCMExt(RW_PCMWrap(rw)) {
+  import Wrap = RW_PCMWrap(rw)
+
+  type M = rw.M
+  function dot(x: M, y: M) : M { rw.dot(x, y) }
+  predicate valid(x: M) { exists y :: rw.Inv(dot(x, y)) }
+  function unit() : M { rw.unit() }
+
+  // Partial Commutative Monoid (PCM) axioms
+
+  lemma dot_unit(x: M)
+  ensures dot(x, unit()) == x
+  {
+    rw.dot_unit(x);
+  }
+
+  lemma valid_unit(x: M)
+  ensures valid(unit())
+  {
+    rw.inv_unit();
+    dot_unit(unit());
+    assert rw.Inv(dot(unit(), unit()));
+  }
+
+  lemma commutative(x: M, y: M)
+  ensures dot(x, y) == dot(y, x)
+  {
+    rw.commutative(x, y);
+  }
+
+  lemma associative(x: M, y: M, z: M)
+  ensures dot(x, dot(y, z)) == dot(dot(x, y), z)
+  {
+    rw.associative(x, y, z);
+  }
+
+  predicate transition(a: M, b: M) {
+    rw.transition(a, b)
+  }
 
   lemma transition_is_refl(a: M)
-  requires transition(a, a)
+  //requires transition(a, a)
   { }
 
   lemma transition_is_trans(a: M, b: M, c: M)
-  requires transition(a, b)
-  requires transition(b, c)
-  ensures transition(a, c)
+  //requires transition(a, b)
+  //requires transition(b, c)
+  //ensures transition(a, c)
   { }
 
   lemma transition_is_monotonic(a: M, b: M, c: M)
-  requires transition(a, b)
-  ensures transition(dot(a, c), dot(b, c))
-  { }
+  //requires transition(a, b)
+  //ensures transition(dot(a, c), dot(b, c))
+  {
+    forall p: M | rw.Inv(rw.dot(rw.dot(a, c), p))
+    ensures rw.Inv(rw.dot(rw.dot(b, c), p)) && rw.I(rw.dot(rw.dot(a, c), p)) == rw.I(rw.dot(rw.dot(b, c), p))
+    {
+      associative(b, c, p);
+      associative(a, c, p);
+      assert rw.Inv(rw.dot(a, rw.dot(c, p)));
+    }
+    assert rw.transition(dot(a, c), dot(b, c));
+    assert transition(dot(a, c), dot(b, c));
+  }
+
+  function I(f: F) : Option<B> {
+    if rw.Inv(f) then (
+      if rw.I(f).Some? then (
+        Some(Wrap.one(rw.I(f).value))
+      ) else (
+        Some(Wrap.unit())
+      )
+    ) else (
+      None
+    )
+  }
+
+  lemma I_unit()
+  ensures I(unit()) == Some(base.unit())
+  {
+    rw.inv_unit();
+  }
+
+  lemma I_respects_transitions(f: F, f': F)
+  //requires transition(f, f')
+  //requires I(f).Some?
+  //ensures I(f').Some?
+  //ensures base.transition(I(f).value, I(f').value)
+  {
+    assert rw.Inv(f);
+    rw.dot_unit(f);
+    rw.dot_unit(f');
+    assert rw.Inv(rw.dot(f, unit()));
+  }
+
+  lemma I_valid(f: F)
+  //requires I(f).Some?
+  //ensures valid(f)
+  {
+    assert rw.Inv(f);
+    rw.dot_unit(f);
+    assert rw.Inv(dot(f, unit()));
+  }
+}
+
+module RWTokens(rw: RW) {
+  // TODO fill in init, transition, withdraw, deposit methods
 }
