concurrency/framework/SSM.i.dfy
@@ -176,4 +176,6 @@ module SSMTokens(ssm: SSM) {
     transition_of_next_with_unit(a.val, expect_b);
     Tokens.transition_update(Tokens.get_unit_shared(a.loc), a, expect_b)
   }
+
+  // TODO more stuff here ...
 }
